coq/Langs/TMMon.v
@@ -1,0 +1,134 @@
+Set Implicit Arguments.
+Require Import Strings.String CSC.Langs.Util CSC.Util.
+
+(** The type used for variable names. *)
+Definition vart := string.
+
+(** References *)
+Inductive loc : Type :=
+| addr : nat -> loc
+.
+Lemma loc_dec (x y : loc) : {x = y} + {x <> y}.
+Proof.
+  destruct x, y, (PeanoNat.Nat.eq_dec n n0); subst; ((now left) + right); congruence.
+Defined.
+(** Types of temporal memory safe events. *)
+Variant event : Type :=
+| Salloc (ℓ : loc) : event
+| Sdealloc (ℓ : loc) : event
+| Suse (ℓ : loc) : event
+| Scrash : event
+.
+#[local]
+Instance event__Instance : TraceEvent event := {}.
+Definition ev_to_tracepref := @Langs.Util.ev_to_tracepref event event__Instance.
+Coercion ev_to_tracepref : event >-> tracepref.
+Definition eventeq (a0 a1 : event) : bool :=
+  match a0, a1 with
+  | Salloc(addr ℓ0), Salloc(addr ℓ1) => Nat.eqb ℓ0 ℓ1
+  | Sdealloc(addr ℓ0), Sdealloc(addr ℓ1) => Nat.eqb ℓ0 ℓ1
+  | Suse(addr ℓ0), Suse(addr ℓ1) => Nat.eqb ℓ0 ℓ1
+  | Scrash, Scrash => true
+  | _, _ => false
+  end
+.
+
+(** Locations *)
+Definition Loc := list loc.
+(** Abstract Store *)
+Record TMSMonitor := {
+  A: Loc ;
+  F: Loc
+}.
+#[local]
+Instance tmsmon__Instance : RuntimeExprClass TMSMonitor := {}.
+
+Definition emptytmsmon : TMSMonitor := {|
+  A := List.nil ;
+  F := List.nil
+|}.
+#[local]
+Notation "∅" := (emptytmsmon) (at level 82).
+
+Definition entails (T1 T2 : TMSMonitor) := forall x, List.In x T1.(F) -> List.In x T2.(F).
+Definition contains (ℓ : loc) (T : TMSMonitor) := List.In ℓ T.(A) /\ ~(List.In ℓ T.(F)).
+Definition notin (ℓ : loc) (T : TMSMonitor) := ~(List.In ℓ T.(F)) /\ ~(List.In ℓ T.(A)).
+Definition extend (ℓ : loc) (T : TMSMonitor) : TMSMonitor := {|
+  A := List.cons ℓ T.(A) ;
+  F := T.(F)
+|}.
+Definition without (T : TMSMonitor) (ℓ : loc) : TMSMonitor := {|
+  A := List.remove loc_dec ℓ T.(A) ;
+  F := List.cons ℓ T.(F)
+|}.
+#[local]
+Notation "T1 '⊆__F' T2" := (entails T1 T2) (at level 82, T2 at next level).
+#[local]
+Notation "ℓ '∈' T" := (contains ℓ T) (at level 82, T at next level).
+#[local]
+Notation "ℓ '∉' T" := (notin ℓ T) (at level 82, T at next level).
+#[local]
+Notation "'{' ℓ '}' '∪' T" := (extend ℓ T) (at level 82, T at next level).
+#[local]
+Notation "T '∖' '{' ℓ '}'" := (without T ℓ) (at level 82, ℓ at next level).
+
+(** Step Relations *)
+Inductive step : CtxStep :=
+| TMS_uninteresting : forall (T__TMS : TMSMonitor),
+    T__TMS ==[]==> T__TMS
+| TMS_use : forall (T__TMS : TMSMonitor) (ℓ : loc),
+    ℓ ∈ T__TMS ->
+    T__TMS ==[Suse ℓ]==> T__TMS
+| TMS_alloc : forall (T__TMS T__TMS' : TMSMonitor) (ℓ : loc),
+    T__TMS' = ({ ℓ } ∪ T__TMS) ->
+    ℓ ∉ T__TMS ->
+    T__TMS ==[Salloc ℓ]==> T__TMS'
+| TMS_dealloc : forall (T__TMS T__TMS' : TMSMonitor) (ℓ : loc),
+    ℓ ∈ T__TMS ->
+    T__TMS' = (T__TMS ∖ { ℓ }) ->
+    T__TMS ==[Sdealloc ℓ]==> T__TMS'
+.
+#[local]
+Existing Instance step.
+Inductive star_step : MultStep :=
+| TMS_refl : forall (T__TMS : TMSMonitor),
+    T__TMS ==[]==>* T__TMS
+| TMS_trans : forall (T__TMS T__TMS' T__TMS'' : TMSMonitor) (a : event) (As : tracepref),
+    T__TMS ==[a]==> T__TMS' ->
+    T__TMS' ==[As]==>* T__TMS'' ->
+    T__TMS ==[Tcons a As]==>* T__TMS''
+| TMS_trans_uninteresting : forall (T__TMS T__TMS' T__TMS'' : TMSMonitor) (As : tracepref),
+    T__TMS ==[]==> T__TMS' ->
+    T__TMS' ==[As]==>* T__TMS'' ->
+    T__TMS ==[As]==>* T__TMS''
+.
+#[local]
+Existing Instance star_step.
+
+(** Definition of Temporal Memory Safety on Traces *)
+Definition tmssafe (As : tracepref) :=
+  forall ℓ, (before eventeq (Salloc ℓ) (Sdealloc ℓ) As
+    /\ ~(before eventeq (Suse ℓ) (Salloc ℓ)) As
+    /\ ~(before eventeq (Sdealloc ℓ) (Suse ℓ)) As)
+.
+(** Definition of Temporal Memory Safety on Traces, using our monitor. *)
+Definition TMS (As : tracepref) :=
+  exists T__TMS, ∅ ==[As]==>* T__TMS
+.
+
+Definition simptmssafe (As : tracepref) :=
+  forall ℓ, before eventeq (Salloc ℓ) (Sdealloc ℓ) As.
+
+(* Show the above are equally strong...? *)
+Theorem TMS_refines_tmssafe As :
+  TMS As -> simptmssafe As.
+Proof.
+  intros [T__TMS H]; induction H; try easy.
+  destruct a as [[ℓ] | [ℓ] | [ℓ] | ].
+  - intros [ℓ0] x Ha.
+    destruct (PeanoNat.Nat.eq_dec ℓ ℓ0); subst.
+    destruct x.
+    + cbn in Ha. rewrite PeanoNat.Nat.eqb_refl in Ha.
+      (*idea: unfold ihstar_step and get witness n, then instantiate with S(n)*)
+    (*apply not_eq_None_Some in Ha as [x Ha].*)
+Admitted.
